$|x^{2} - 5x|$=6

$|x^{2} + x- 1| = 2x - 1$

$|3x - 6| = 0|$

$|4x + 5| = -3$

$|2 - |5 - x|| = 2$

***
$|x| + |x - 1| = 1$

$|3x - 8| + |2 - 4x| + |x -5| = 7$

$7x^2 + 2|x - 1| + 2 = 0$

 
 ***
$\dfrac{|x^3| - |5x|}{\sqrt{2x^2-4x-1}-|x|+2}$

$|\dfrac{x - 1}{x - 2}| = |\dfrac{x + 1}{x + 2}|$

$x^2 + |x| - 6 = 0$

$(4|x + 1| + \dfrac{1}{2} )^2 = 11(x + 1)^2 + \dfrac{5} {4}$

$3x^4 + x^2 - 8x - 4x^2|x - 4| + 16 = 0$

$|5x - 2| = 4$

$|3 - 7x| = -2$

$|3 -4x| = |5 - 6x|$

$|14 - 2x| = 3 - 5x$

$7x^2 + 2|x-1| + 2 = 0$

$|3x - 8| + |2 -4x| + |x-5| = 7$

$|5x + 3| = 1$

$|2x+ 5| + |2x - 3| = 8$

$|x^2 + 2x| - |2 -x| = |x^2 - x|$

$2|x+6| - |x| + |x- 6| = 18$

$|3x - 2| = 1$

$|101x + 4| = -1$

$|x^2 - 3x| = 0$

$||x+1| - 4| = 3$

$|||x-5| -5| -5| = 5$

$|8 - |x-2|| = 7$

$|x+1| + |5 - x| = 2$

$|1-x| + |x+ 2| = 3$

$|8 + x| + |x + 7| = 10$

$||2x + 3| - 4| = x$

$|2x - x^2 + 3| = 1$

$|1 - |1-x|| = 0.5$

$|x - 3 - |x|| = 4$

$|3 - 2x| = 3x$

$|x^2 + 2x - 3| = x^2 + x -20$

$|4 - y| = |2y + 1|$

$||x| - 2| = |x|$

$|x^2 - 1| = (x-1)(x+1)$

$|\dfrac{2-x}{x-3}| = \dfrac{x-2}{x-3}$

