## Решение уравнений и линейных неравенств.

$x^2 + \dfrac{4x^2}{(x+2)^2} = 5$

$\dfrac{1}{(x^2 - 2x)^2 + 1} + \dfrac{2}{(x-2)^2 + 2} + \dfrac{3}{(x^2 - 3x + 2)^2 + 3} = 3$

$\dfrac{1}{x} + \dfrac{1}{x+2} + \dfrac{1}{x+3} + \dfrac{1}{x+5} = 0$

$x^2 + (\dfrac{x}{2x -1})^2 = 2$

$x^4 - 10x^2 + 25 = 0$

$\dfrac{1}{(x-3)^2} + \dfrac{9}{(x+3)^2} - \dfrac{6}{x^2 - 9}$

$(\dfrac{x}{x + 1})^2 - 5\dfrac{x}{x + 1} + 6 = 0$

$\dfrac{x}{x-2} + \dfrac{5}{x} = 4$

$\dfrac{x^2 - 3x +2}{36} = 0$

$\dfrac{x - 3 }{x - 5} + \dfrac{1}{x} = \dfrac{x + 5}{x^2 - 5x}$

***

$5(x-1) + 7 \leq 1 -3(x+2)$

$a + 2< 5(2a + 8) + 13(4 - a)$

$x -2 \geq 4.7(x-2) - 2,7 (x-1)$

$\dfrac{1}{3}x > 6$

$4(b -1.5) - 1.2 \geq 6b -1$

$1.7 - 3(1 -m) \leq -(m - 1,9)$
