\documentclass[12pt, a4paper]{article}
\usepackage{../../../../../style}
\begin{document}
	
	\lhead{Группа 91} \chead{Модуль 6} \rhead{Школа <<Симметрия>>} \cfoot{}
	\begin{center}
		\Large
		\textbf{Занятие №6}
	\end{center}
	\begin{enumerate}
		\item Вычислить:
		\begin{multicols}{2}
			\begin{enumerate}[label=\asbuk*)]
				\item $\sqrt{27\cdot12}$
				\item $\sqrt{40\cdot55\cdot22}$
				\item $\sqrt{245\cdot27\cdot60}$
				\item $\sqrt{98}\cdot\sqrt{50}$
			\end{enumerate}
		\end{multicols}
		\item Решить уравнения:
		\begin{multicols}{2}
			\begin{enumerate}[label=\asbuk*)]
				\item $x(x-1)=0$
				\item $x^2-4x=0$
				\item $2x^2=5+3x$
			\end{enumerate}
		\end{multicols}
		\item Упростить выражение: $$\dfrac{x^2-y^2}{(x+y)^2}:\dfrac{6x-6y}{3x+3y}$$
		\item Упростить выражение: $$\dfrac{a^2+ab}{4a^2-4b^2}\cdot\dfrac{2a^3+2b^3}{a^2-ab}$$
		\item Упростить выражение: $$\dfrac{6a}{4-9a^2}+\dfrac{1}{3a-2}$$
		\item Решить систему уравнений:
		$$\left\{
		\begin{array}{l}
			x+y-3=0,\vspace{0,2cm}\\
			x-y+1=0
		\end{array}
		\right.$$
		\item Решить систему уравнений:
		$$\left\{
		\begin{array}{l}
			x+2y-3=0,\vspace{0,2cm}\\
			2x-3y=-8
		\end{array}
		\right.$$
		\item Решить уравнения:
		\begin{enumerate}[label=\asbuk*)]
			\item $\dfrac{x^2}{5}-\dfrac{2x}{3}=\dfrac{x+5}{6}$
			\item $(x+3)(x-2)+(x+2)^2=3x+10$
		\end{enumerate}
	\end{enumerate}
\end{document}