$\dfrac{x}{x-2} + \dfrac{5}{x} = 4$

$\dfrac{7}{x} = -4x + 1$

$x - 7 = \dfrac{x+8}{12}$

$\dfrac{x^2 - 3x +2}{36} = 0$

$\dfrac{2x^2 + x - 3}{3x^2 - 2x - 1} = 0$

$\dfrac{x^2 -12}{x - 3} = \dfrac{x}{3 -x}$

$\dfrac{2x - 3}{x} - \dfrac{1}{x + 2} = \dfrac{4x - 6}{x^2 + 2x}$

***

$\dfrac{1}{x^2 - 4x + 4} - \dfrac{4}{x^2 - 4} = \dfrac{1}{x+2}$

$\dfrac{x - 3 }{x - 5} + \dfrac{1}{x} = \dfrac{x + 5}{x^2 - 5x}$

$\dfrac{x^2 - 9x + 20}{x - 5} = 0$

$(\dfrac{x}{x + 1})^2 - 5\dfrac{x}{x + 1} + 6 = 0$

$\dfrac{1}{x^2 + 3x - 3} + \dfrac{2}{x^2 + 3x + 1} = \dfrac{7}{5}$

$\dfrac{x}{x + 4} + \dfrac{x + 4}{x - 4} = \dfrac{32}{x^2 - 16}$

$\dfrac{x-2}{x+3} - \dfrac{30}{x^2 - 9} = 3$

$\dfrac{2x^2 - 3x - 5}{x + 1} = 0$

$\dfrac{x^2 + 3x}{2} + \dfrac{x - 3x^2}{8} = 2x$

$\dfrac{x^2 - 1}{x + 5} = \dfrac{5 -x}{x + 5}$

$\dfrac{1}{3x + 1} - \dfrac{1}{9x^2 + 6x + 1} = 2$

$\dfrac{5}{x - 2} + 1 = \dfrac{14}{x^2 - 4x + 4}$

$\dfrac{5}{y+ 3} - \dfrac{3}{y} = \dfrac{2 - y}{y^2 + 3y}$

$\dfrac{4y + 7}{2y - 3} - \dfrac{y - 3}{2y + 3} = 1$

$\dfrac{3x - 9}{x -1} + \dfrac{x + 6}{x + 1} = 3$

$\dfrac{3}{x + 2} - \dfrac{3}{2 - x} = \dfrac{2}{x^2 - 4}$

$\dfrac{3}{1 - 4y^2} + \dfrac{4}{2y^2 + y} = \dfrac{3}{4y^2 + 4y + 1}$

$\dfrac{1}{(x-3)^2} + \dfrac{9}{(x+3)^2} - \dfrac{6}{x^2 - 9}$

$\dfrac{2x - 7}{x- 4} + \dfrac{x+2}{x+1} = \dfrac{x+6}{(x-4)(x+1)}$

$\dfrac{2x+ 1}{3} - \dfrac{4x - x^2}{12} = \dfrac{x^2 - 4}{9}$

$\dfrac{x^2 + 3x}{x -4} = \dfrac{x^2 -x}{4 - x}$

$\dfrac{2y^2 + 5y + 2}{y^2 - 4} =1$

$\dfrac{9x + 3}{1 + 3x} = x - 7$

$\dfrac{2x + 3}{x+2} = \dfrac{3x + 2}{x}$

$\dfrac{7a - 6}{a^3 + 27} = \dfrac{1}{a^2- 3a + 9} - \dfrac{1}{a + 3}$

$\dfrac{y + 3}{9y^2 + 3y + 1} + \dfrac{3}{27y^3 - 1} = \dfrac{1}{3y - 1}$

$\dfrac{3}{1 - 4y^2} + \dfrac{4}{2y^2 + y} = \dfrac{3}{4y^2 + 4y + 1}$

$\dfrac{1}{(x^2 - 2x)^2 + 1} + \dfrac{2}{(x-2)^2 + 2} + \dfrac{3}{(x^2 - 3x + 2)^2 + 3} = 3$

$x^2 + \dfrac{4x^2}{(x+2)^2} = 5$

$\dfrac{1}{x} + \dfrac{1}{x+2} + \dfrac{1}{x+3} + \dfrac{1}{x+5} = 0$

$\dfrac{4x}{4x^2 - 8x + 7} + \dfrac{3x}{4x^2 - 10x + 7} - 1 = 0$

$\dfrac{2x}{3x^2 - x + 2} - \dfrac{7x}{3x^2 + 5x + 2} - 1= 0$

