$\sqrt{x^2 - 5} = 2$

$\sqrt{x - 2} = x - 8$

$\sqrt[3]{x^2 - 5} = 0$

$x - \sqrt{x} - 2 = 0$

***

$\sqrt{x^2 - x - 3} = \sqrt{x}$

$\sqrt{x} - \dfrac{3}{\sqrt{x}} + 2 = 0$

$\sqrt{x -13} = \sqrt{x + 8} - 3$

$\sqrt{5 - x} + \sqrt{25 - x^2} = 0$

$\sqrt{x^2 + x} + \sqrt{x^2 + x + 5} = \sqrt{2x^2 + 2x + 17}$

$\sqrt{\dfrac{20 + x}{x}} + \sqrt{\dfrac{20 - x}{x}} = \sqrt{6}$

$\sqrt{2 - \sqrt{x +1}} + \sqrt{2 + \sqrt{x +1}} = 2\sqrt{x}$

$\sqrt{4-x^2} + \sqrt{x - 2} = \sqrt{x + 7} - \sqrt{4x -1}$

$\sqrt{x^2 + 2x + 1} - \sqrt{x^2 + 2x - 27} =2$

$5 + \sqrt{6- x} = 7$

$\sqrt{5 + \sqrt{x-4}} = 3$

$\sqrt{x+1} + \sqrt{2x +3} = 1$

$\sqrt{3x + 4} + \sqrt{x+2} = 8$

$\sqrt{22-x} - \sqrt{ 10 -x} = 2$

$2\sqrt{x+18} + \sqrt{4x - 3} = 15$

$\sqrt{2x + 1} + \sqrt{x-3}  = 2\sqrt{x}$

$\sqrt{1+ x\sqrt{x^2 +12}} = 1+x$

$\dfrac{2}{x} + 2 = \sqrt{4+x\sqrt{36 + x^2}}$

$1 - \dfrac{1}{x} = \sqrt{1 - \dfrac{1}{x}\sqrt{4 - \dfrac{7}{x^2}}}$

$\dfrac{5}{x+\sqrt{5 + x^2}} - \dfrac{5}{x - \sqrt{5 + x^2}} = 6$

$\dfrac{4}{x+\sqrt{4 - x^2}} + \dfrac{4}{x - \sqrt{4 -x^2}} = \dfrac{12}{7}$

$\dfrac{x-1}{1 + \sqrt{x}} = 4 - \dfrac{ 1- \sqrt{x}}{2}$

$x + \sqrt{ 16x + x^2} = 8$

$\sqrt{17 - \sqrt{x-8}} = 4$

$\sqrt{2x -1} + \sqrt{x-1} = 1$

$\sqrt{2x + 1} + \sqrt{7x - 27} = \sqrt{3x + 4}$

$\dfrac{3 + x}{3x} = \sqrt{\dfrac{1}{9} + \dfrac{1}{x}\sqrt{\dfrac{4}{9} + \dfrac{2}{x^2}}}$

$\dfrac{5x -1}{\sqrt{5x} + 1} = 1 + \dfrac{\sqrt{5x} - 1}{2}$

$\dfrac{5}{x + \sqrt{5 - x^2}} + \dfrac{5}{x - \sqrt{5 - x^2}} = \dfrac{20}{3}$

$\dfrac{1}{1 - \sqrt{1 - x^2}} - \dfrac{1}{1 + \sqrt{1 - x^2}} = \dfrac{\sqrt{3}}{x^2}$

$\log_{\frac{1}{26}}(26x - 2) \leq 0$

$\log_{28}x + \log_{28}(x - 27) < 1$

$\log_{31}(31x + 2) \leq 1$

$\log_{\frac{1}{11}}(2x - 1) + \log_{\frac{1}{11}}x > 0$

$\log_{\frac{1}{8}}(8x - 2) \geq 0$

$\lg x + \lg(x - 9) < 0$

$\log_{33}(33x + 2) \leq 0$

$\log_{\frac{1}{9}}(2x - 1) + log_{\frac{1}{9}}x > 0$

$\log_{\frac{1}{6}}(6x - 2) \geq 0$

$\log_8x + log_8(9x - 7) < 1$

$\log_{32}(35x + 2) \leq 1$

$\log_{\frac{1}{7}}(2x - 1) = log_{\frac{1}{7}}x > 0$

$\log_4x + \log_4(x-3) < 1$

$\log_{12}x + \log_{12}(x -11) < 1$

$\log_3\dfrac{1}{x} + \log_3(x^2 + 3x - 9) \leq \log_3(x^2 + 3x + \dfrac{1}{x} - 10)$

$9\log_7(x^2 + x - 2) \leq 10 + \log_7\dfrac{(x-1)^9}{x+2}$

$\log_2(x^2 - 4) - 3\log_2\dfrac{x+2}{x-2} > 2$

$\dfrac{log_2x - 5}{1 - 2log_2x} \geq 2log_2x$

$\log_3(x^2 - x - 3) + \log_3(2x^2 + x - 3) \geq \log_3(x^2 -2)^2 + 2 + \log_{\frac{1}{3}}4$

$\dfrac{\lg(5y^2 -2y + 1)}{\lg(4y^2 - 5y + 1)^3} \leq \dfrac{\log_{5^3}7}{\log_57}$

$\dfrac{\ln(3y^2 - 2y + 1)}{\ln(5y^2 - 6y + 1)^5} \geq \dfrac{log_{5^3}7}{log_57}$
$\dfrac{lg(3x + 2\sqrt{x} - 1)}{lg(5x + 3\sqrt{x} - 2)^5} \geq \dfrac{log_{32}11}{log_211}$

