$3x + 15 = 0$

$-8x +2x = 6x - 4$

$2(3x -1) = 4(x +3)$

$2x + 2 = -3$

$-x - 2 + 3(x-3) = 3(4 - x) - 3$

$3(2 + 1.5x) = 0.5x + 24$

$4(x + 2) - 0.7 = 2(2x + 4) + 0.3$

$9x + 13 = 7x + 5$

$-5(x + 1) = -20$

$4(x+7) = 2(x+ 6)$

$2x + 5 = 2(x+ 6)$

$3(x+ 2) + x = 6 + 4x$

$2x + 5 = 2(- x + 1) +11$

$6y - 3(y-1) = 4 + y$

$4(x-1) - 3 = -(x+7) + 8 $

$-2(5y-9)+2 = 15 + 7(-x -2)$

$12 + 4(x-3) - 2x = (5 - 3x) + 9$

$-4x + 1 = 4(1 - x)$

$2(5x+ 8) - 3 = 19$

***

$0.8x + 1.4 = 1.4x - 2.6$

$2\dfrac{2}{5}x + 3\dfrac{2}{15} = 3\dfrac{1}{5}x + 2\dfrac{1}{3}$

$\dfrac{1}{4} - \dfrac{1}{3}x = 4\dfrac{1}{4} - 3x$

$2.4(6 - 3x) + 4.3 = 1.7 - 5.2x$

$5(0.1x - 0.5) + 1.6 = 0.4(x-3)$

$1.2(23x - 3.1) + 3 = 3.14x - 1.1$

$\dfrac{x-2}{3} - \dfrac{3x}{2} = 5$

$\dfrac{6x -1}{5} - \dfrac{2-x}{4} = \dfrac{3x+2}{2}$

$\dfrac{5x + 3}{4} - \dfrac{8 -5x}{6} = 4 + 3x$

$(9.1 - x) - 2.8 = 2.9$

$(x-5.6) : 12 = 3.7$

$(x + 2.1) \cdot 4 = 15.2$

$3.4x - 9x = 1.6$

$8.1x : x - 0.7 = 0.3$

$12x + 14x + 4.2 = 12$

$(9.8 - x) : 9 = 0.7$

$x - 3.8 = 8.04$

$x - 6.5 = 12.25$

$9.71 - y = 3.031$

$x + 1.2 = 11.28$

$23.175 - z = 15.02$

$x + 17.051 = 62.3$

$18.63 : (4.5 + 1.2x) = 2.3$

$6.7 \cdot (7.9 - y) = 28.81$

$(x - 18.2) + 3.8 = 15.6$

$\dfrac{1.4x - 3.5}{0.5} = \dfrac{2.3x - 9}{-1.5}$

$\dfrac{7}{9}x - \dfrac{5}{18}x + \dfrac{1}{4}x = \dfrac{1}{6}$