$x \geq - 2$

$x \leq 3$

$x > 8$

$x <- 5$

$x > 0.3$

$x \leq - 8.1$

$-1.5 \leq x \leq 4$

$-2 < x < 1.3$

$-5 \leq x \leq -3\dfrac{1}{3}$

$2 < x \leq 6.1$

$3x > 15$

$-4x < -16$

$-x \geq 1$

$11y \leq 33$

$12y < 1.8$

$27b \geq 12$

$-6x > 1.5$

$15x \leq 0$

$0.5y > -4$

$2.5a > 0$

$\dfrac{1}{3}x > 6$

$-\dfrac{1}{7}y < -1$

$2x < 17$

$5x \geq -3$

$-12x < -48$

$-x < -7.5$

$30x > 40$

$27b \geq 12$

$-6x > 1.5$

$15x \leq 0$

***

$5(x-1) + 7 \leq 1 -3(x+2)$

$4(a+8) - 7(a-1) < 12$

$4(b-1.5) - 1.2 \geq 6b -1$

$1.7 - 3(1 -m) \leq -(m - 1.9)$

$4x > 12(3x - 1) - 16(x+1)$

$a + 2< 5(2a + 8) + 13(4 - a)$

$6y -(y + 8) - 3(2-y) \leq 2$

$4(b -1.5) - 1.2 \geq 6b -1$

$4(2 -3x) - (5 -x) > 11 - x$

$2(3 -z) - 3(2 + z) \leq z$

$1 > 1.5(4 - 2a) + 0.5(2 -6a)$

$2.5(2 -y) - 1.5(y -4) \leq 3 - y$

$x -2 \geq 4.7(x-2) - 2.7 (x-1)$

$3.2(a-6) - 1.2a \leq 3(a -8)$ 

***

$\dfrac{\sqrt{4 - x^2}}{x-1} \leq \dfrac{\sqrt{4-x^2}}{x+1}$

$\lg(3x + 2) + ( 4x - 3)^2(5x - 4)^4(6x -5)^5 \geq \lg(3x + 2)$

*$\dfrac{(|x-3| - x - 13)(\sqrt{x+6} - 2x + 3)}{x^2 - 16} \leq 0$

***
$(x-3)^3(x-4)^4(x-5)^5 \geq 0$

$x(x+1)(x+2)^2(x+3)^3 \leq 0$

$\dfrac{(2x -13)(2 -5x)^4(x-7)^2}{x^2 - 49} \leq 0$

$\dfrac{1}{x-2} + \dfrac{1}{x+2} \leq \dfrac{2}{x+3}$

$(x^2 - 8x + 14)(\sqrt{x+6} -3)(x - \sqrt{2x + 3}) \geq 0$

$(x^2 - 8x +15)(\sqrt{x+10} - 4)(x- \sqrt{ 5x + 6}) \leq 0$

$\dfrac{(\sqrt{x+4} + x - 8)(\sqrt{x+5} + x - 7)}{x + \sqrt{x + 6} - 6} \leq 0$

$\dfrac{(\sqrt{x+8} + x - 4)(\sqrt{x+7} + x - 5)}{x + \sqrt{x + 5} - 7} \leq 0$

$(2x - |x-3| - 7)(3x - |x+2| - 8 ) \geq 0$

$(4x - |3x+ 1| - 8)(5x - |4x - 1| - 3) \geq 0$

$2 + (\log_3(x+2) - 2)(\log_2(x+3) - 3) \geq \log_3(x+2)$

$\sqrt[7]{4x - 9} \geq 0$

$\sqrt[3]{5 -2x}  > 0$

$\sqrt[13]{5x +9} \leq 0$

$\sqrt[5]{-11 - 4x} <0$

$\sqrt[6]{7x - 8} \geq 0$

$\sqrt{7 - 6x} < 0$

$\sqrt[4]{-3x - 5} \leq 0$

$\sqrt[18]{10x - 9} < 0$

$(7x -1)^{\frac{1}{7}} \geq 0$

$\sqrt[7]{7x - 8} > 0$

$\sqrt[16]{4x -4x^2} \geq 0$

$\sqrt{x^2 -5x +1} > 0$

$\sqrt{x^2 - 4x - 9} > 6$

$\sqrt[14]{6x - 9x^2} \geq 1$

$\sqrt[4]{8 -x} \leq 3$

$|2x^2 -13| \geq 5$

$|x^2 - 10x| < 24$

$|9x^2 - 12x -1| \geq 4$

$|2x^2 + 4x - 39| \leq 9$

***

$\left\{
  \begin{array}{c}
     |2x -5| & \geq & 15 \\
     |5x -2| & \leq & 48 \\
  \end{array}
\right.$

$\left\{
  \begin{array}{c}
     |9x^2 -5| & \leq & 4 \\
     |3x -2| & \geq & 1 \\
  \end{array}
\right.$

$\left\{
  \begin{array}{c}
     |x^2 -100| & \leq & 96 \\
     |x^2 -13x| & \leq & 30 \\
  \end{array}
\right.$

$\left\{
  \begin{array}{c}
     |5x^2 -37x| & \leq & 42 \\
     |x^2 -6x + 4| & \leq & 4 \\
  \end{array}
\right.$

$\left\{
  \begin{array}{c}
     |x^2 - 25| & \leq & 24 \\
     |x^2 - 5x| & \leq & 6 \\
  \end{array}
\right.$

$\left\{
  \begin{array}{c}
     |4x^2 - 41x| & \leq & 45 \\
     |x^2 - 8x - 1| & \leq & 8 \\
  \end{array}
\right.$

$|2x^2 - 5| \geq 3$

$|x^2 - 5x| < 6$

$|4x^2 - 12x - 1| \geq 6$

$4 \leq |2x - 7| \leq 12$

$|x^2 - 4x - 25| > 20$

$18 \leq |x^2 + 2x - 17| \leq 31$

$|4x - 9| > 0$

$|10x - 11| \leq 12$

$|5x + 4| \geq 3$

$|2x^2 + 5x - 18| \leq 0$

$|x^2 - 50| \leq 14$

$|3x^2 - x| \geq 0.08$

$|x^2 - x -4| < 2$

$\dfrac{3}{x^2 - 3x - 18} > \dfrac{4}{x^2 - 3x - 18}$

$\dfrac{(2x -19)^3(7 -5x)^6(x-10)^2}{x^2 - 100} \leq 0$

$\dfrac{4}{(3x + 4)^2} - \dfrac{16}{3x + 4} + 15 > 0$

$\dfrac{x^2 - 5x - 3}{x - 5} + \dfrac{7}{x-9} \leq x$

$x^3 + 9x^2 + \dfrac{40x^2 + x - 5}{x-5} ] \leq 1$

$\dfrac{x^3 - 4x^2 + 2x + 4}{x^2 - 4x} \leq x - \dfrac{1}{x} + \dfrac{1}{x-2}$

$\dfrac{3}{x^2 + 8x + 17} + \dfrac{4}{x^2 + 8x + 18} \geq 5$

$\dfrac{2}{x^2 + 10x + 27} + \dfrac{5}{x^2 + 10x + 26} \geq 6$

$\dfrac{x^2 - 5x + 4}{x-5} \leq x + \dfrac{2}{x-3}$


$\dfrac{x^2 - 2x - 1}{x-2} + \dfrac{x^3 - 4x^2 - 3}{x-4} \leq x + x^2$

$\dfrac{x^2 - 6x -1}{x -6} + \dfrac{5}{x-10} \leq x$

$\dfrac{x^2 - 3x -5}{x-4} + \dfrac{x^2 - 6x + 3}{x-6} \leq 2x + 1$

$\dfrac{12x + 9}{x-7} + \dfrac{62}{x^2 - 9x + 14} + \dfrac{8}{x-2} \leq 0$

$x^3 + 6x^2 + \dfrac{40x^2 + x - 8}{x-8} \leq 1$

$\dfrac{ x^2 - 7x - 3}{x-7} + \dfrac{7}{x-11} \leq x$

$\dfrac{x^2 - 6x + 2}{x-7} + \dfrac{4x - 29}{x-9} \leq x+3$

$\dfrac{x^2 - 8x + 4}{x-7} + \dfrac{3x - 26}{x-11} \leq x+2$

$\dfrac{3}{x^2 + 5} \geq \dfrac {2x}{x^2 + 5}$

$\dfrac{4x^2}{4x + 3} < -\dfrac{7}{4x + 3}$

$\dfrac{2}{5x - 4} \leq \dfrac {3}{5x - 4}$

$x^2 \geq \dfrac{16x + 64}{x + 4}$

$\dfrac{2}{x-3} \leq 1$

$\dfrac{3}{x-4} \leq 1$

$\dfrac{2}{x^2 + 4} \leq \dfrac{3x}{x^2 + 4}$

$\dfrac{5x^2}{5x - 4} > -\dfrac {9}{5x -4}$

$\dfrac{4}{3x +4} \geq \dfrac{3}{3x +4}$

$x^2 \leq \dfrac{9x - 27}{x-3}$

$\dfrac{3x^2}{2x+5} \leq 0$

$\dfrac{(x+7)^2}{x^2 - 36} \leq 0$

$\log_{x^2+x}(x^2 - 2x + 1) \leq 1$

$\log^2_2(3x-1) + \log^2_{3x-1}2 - \log_2(3x-1)^2 - \log_{3x-1}4 + 2 \leq 0$

$\log_{6x^2 - 5x + 1}2 > \log_{\sqrt{6x^2 - 5x + 1}}2$

$(x-1)\log_{x+3}(x +2) \cdot \log_3(x+3)^2 \leq 0$

$\log_216x \geq \log_{0.5x}2 \cdot \log_416x^4$

$\log_{\log_x2x}(9x - 4) \geq 0$

$\log_{x^2}(x-1)^2 \leq 1$

$\log_{2x}0.25 \geq \log_232x - 1$

$\log_{4-x}\dfrac{(x-4)^8}{(x+5)} \geq 8$

$x^2\log_{25}x \geq \log_{25}x^3 + x\log_5x$

$\log^2_3x + 2 > 3\log_3x$

$2^{\log^2_2x} + x^{\log_2x} \leq 256$

$\log^2_2x + 6 \geq 5\log_2x$

$2\log_9(4x^2 + 1) \geq \log_3(3x^2 + 4x + 1)$

$x \cdot \log_4(5 - 3x - x^2) \geq 0$

$\lg^2\dfrac{(x+2)^2(x+5)}{5} < \lg^2\dfrac{x+5}{20}$

$\log_2\dfrac{8}{x} - \dfrac{10}{log_216x} \geq 0$

$\log^2_5(25-x^2) - 3\log_5(25 - x^2) + 2 \geq 0$

$\dfrac{5\lg^2x}{\lg^2x-1} \geq 1$

$\log^22(4 + 3x - x^2) + 7\log_{0.5}(4 + 3x - x^2) + 10 > 0$

$\log_{x+1}(x-1) \cdot \log_{x+1}(x+2) \leq 0$

$(\log_2(x+4.2) + 2)(\log_2(x+4.2) - 3) \geq 0$

$3\log_{11}(x^2 + 8x - 9) \leq 4 + \log_{11}\dfrac{(x-1)^3}{x+9}$

$\log_{\frac{\sqrt2 + \sqrt{13}}{5}}4 \geq \log_{\frac{\sqrt2 + \sqrt{13}}{5}}(5 - 2^x)$

$(5x - 13) \cdot \log_{2x - 5}(x^2 - 6x + 10) \geq 0$

$\lg^4x - 4\lg^3x + 5\lg^2x - 2\lg{x} \geq 0$

$1 + \log_6(4-x) \leq \log_6(16 - x^2)$

$\log^2_3(25 - x^2) - 3\log_3(25 - x^2) + 2 \geq 0$

$\log_{11}(8x^2 + 7) - \log_{11}(x^2 + x + 1) \geq \log_{11}(\dfrac{x}{x+5} + 7)$

$\log_2(4x^2 - 1) - \log_2x \leq \log_2 (5x + \dfrac{9}{x} - 11)$

$\log_{\frac{1}{3}}(\log_2(x^2 - 9) - 2) \geq -1$

$\log_4(6-6x) < \log_4(x^2 - 5x + 4) + \log_4(x+3)$

$\log_6(21 - 7x) \geq \log_6(x^2 - 8x + 15) + \log_6(x+3)$

$\log_2((x-1)(x^2 + 3)) \leq \log_2(4x - x^2 - 3) + \log_2(5 - x)$

$\dfrac{\log_5(3x - 13)}{\log_5(x-4)} \geq 1$

$\log_3((2-x)(x^2 + 5)) \geq \log_3(x^2 - 5x + 6) + \log_3(4-x)$

$x^2\log_{243}(4-x) \leq \log_3(x^2 - 8x + 16)$

$\dfrac{2}{\log_(2x -2)} + \dfrac{3}{\log_2}(4x - 4) \leq \dfrac{8}{\log_327 + \log_2(x-1)}$

***
$\sqrt{3x +2} > 1$

$\sqrt{x^2 + 17x} < 4$

$x^2 \geq 8\sqrt{x}$

$\sqrt{5x + 7} < \sqrt{2 - 3x}$

$\sqrt{x^2 - 3} \geq \sqrt{4x-6}$

$\sqrt{3 -7x} < \sqrt{6x - 8}$

$(x-2)\sqrt{x-1} \geq 0$

$(x+3)\sqrt{2-x} \leq 0$

$(3x^2 - 16x + 21)\sqrt{2x+5} \leq 0$

$(5x^2 + 17x + 14) \sqrt{4-3x} \leq 0$

$(5x - 7)\sqrt{x^2 - 9x + 14} \leq 0$

$\dfrac{6-2x}{\sqrt{x^2 + 7x + 12}} < 0$

$\dfrac{\sqrt{x+3} - 1}{5 - \sqrt{x+3}} \geq 0$

$x^2 + 5x - \sqrt{x^2 + 5x + 4} + 2 < 0$

$\sqrt{15-x} \leq x+5$

$\dfrac{2x + 1}{x} - 2\sqrt{2 + \dfrac{1}{x}} \geq 3$

$x-9 < 3\sqrt{x+1}$

$\sqrt{25x^2 - 10x + 1} < 1$

***

$2^x \leq 4$

$5^x \geq 0.04$

$9^x < 27$

$(\dfrac{1}{36})^x < 6$

$(2.5)^x < 0.4$

$(3.45)^x > 1$

$3^{x^2 - 4x + 6} \leq 9$

$25^x \cdot 125^x \geq 0.2$

$2^{x^2 + 5x} < (0.5)^{-5x - 16}$

$8^{x^2} > 2^{x+2}$

$15^x < 25 \cdot 3^x$

$4^x \cdot 2^{x^2} \geq 8$

$7^{x^2 - 7x + 12} < 49$

$(\dfrac{1}{13})^{5 + x - 6x^2} > 169$

$\left\{
  \begin{array}{c}
     12^x  <  144 \\
     144^x > 12 \\
  \end{array}
\right.$

$\left\{
  \begin{array}{c}
    4^{x -47}   <  64 \\
     7^{x + 47} > \dfrac{1}{49}  \\
  \end{array}
\right.$

$\left\{
  \begin{array}{c}
    \sqrt[14]{14^x} > 14  \\
     \sqrt[16]{16^x} < 16  \\
  \end{array}
\right.$

$\left\{
  \begin{array}{c}
    14^{x-6} > 2 \cdot 7^{x-6}   \\
     14^{x-16} < 7 \cdot 2^{x-16}   \\
  \end{array}
\right.$

$(0.04)^x \cdot 2^{x^2} + 5^{x^2} \cdot 2^x \leq 10{x^2} + (0.08)^x$

$4^x - 7 \cdot 2^x + 10 \leq 0$

$3 \cdot 9^{x^2 - 1} - 12 \cdot 3^{x^2 - 2} + 1 \geq 0$

$7^{2x^2 - 8x + 7} - 10 \cdot 14^{x^2 - 4x + 3} + 3^{2x^2 - 8x + 7} \geq 0$

$\dfrac{80}{(5^{2 - x^2} - 5)^2} + \dfrac{16}{5^{2-x^2} - 5} \leq 1$

$\left\{
  \begin{array}{c}
  \sqrt{x -7} \leq 6   \\
     \sqrt{23 -x} \geq 4  \\
  \end{array}
\right.$

$\left\{
  \begin{array}{c}
     \sqrt{x-3} \leq 5  \\
     (x^2 - 8x + 15)^{\frac{1}{15}} \geq 0  \\
  \end{array}
\right.$

$\left\{
  \begin{array}{c}
    (7x -6)^{0.2} \geq 1  \\
     (6x -5)^{0.1} \leq 1  \\
  \end{array}
\right.$

$\left\{
  \begin{array}{c}
      \sqrt{x-3} \leq 2\\
    \sqrt{12 -x} \geq 3 \\
  \end{array}
\right.$

$\left\{
  \begin{array}{c}
    14^{x-6} > 2 \cdot 7^{x-6}   \\
     14^{x-16} < 7 \cdot 2^{x-16}   \\
  \end{array}
\right.$

$\left\{
  \begin{array}{c}
    (8x -15)^{0.25} \geq 1  \\
     (4x - 7)^{0.5} \leq 1   \\
  \end{array}
\right.$

$\sqrt{x^2 + 17x -2} > 4$

$\sqrt{x^2 + 6x - 7} \leq 3$

$(6x -5)^{\frac{1}{65}} < 1$

